Fix breakage in end2end due to moved function name

src/Bedrock/Group/ScalarMult/CSwap.v
@@ -514,9 +514,11 @@ Section __.
   Import SizedListArrayCompiler.
   Import LoopCompiler.
   Hint Extern 10 (_ < _) => lia: compiler_side_conditions.
-    
-    Instance spec_of_cswap : spec_of "felem_cswap" :=
-      fnspec! "felem_cswap" mask ptr1 ptr2 / c1 c2 R,
+
+  Definition felem_cswap := "felem_cswap".
+  
+    Instance spec_of_cswap : spec_of felem_cswap :=
+      fnspec! felem_cswap mask ptr1 ptr2 / c1 c2 R,
         (*TODO: if b then bw should be all 1s*)
         { requires tr mem :=
             (mask = word.of_Z 0 \/ mask = word.of_Z 1) /\
@@ -531,7 +533,7 @@ Section __.
 
   Import LoopCompiler.
   Derive cswap_body SuchThat         
-           (defn! "felem_cswap" ("mask", "a1", "a2") { cswap_body },
+           (defn! felem_cswap ("mask", "a1", "a2") { cswap_body },
              implements cswap_low)
            As cswap_body_correct.
   Proof.
@@ -581,7 +583,7 @@ Section __.
            Locals := l;
            Functions := functions }>
         cmd.seq
-          (cmd.call [] "felem_cswap" [expr.var mask_var; expr.var lhs_var; expr.var rhs_var])
+          (cmd.call [] felem_cswap [expr.var mask_var; expr.var lhs_var; expr.var rhs_var])
           k_impl
         <{ pred (nlet_eq [lhs_var; rhs_var] v k) }>.
   Proof.
@@ -667,6 +669,6 @@ End __.
 
 Hint Resolve compile_felem_cswap : compiler.
 
-(* TODO: why doesn't `Existing Instance` work? is it the raw string? *)
-Hint Extern 1 (spec_of "felem_cswap") =>
+(* TODO: why doesn't `Existing Instance` work? *)
+Hint Extern 1 (spec_of felem_cswap) =>
        (simple refine (spec_of_cswap)) : typeclass_instances.
